Better handling of array_copy.

HOL/DataStrs/Reverse_Func.thy
@@ -4,6 +4,7 @@ begin
 
 section {* Results about nth *}
 
+setup {* register_wellform_data ("xs ! i", ["i < length xs"]) *}
 setup {* add_rewrite_rule @{thm List.nth_append} *}
 setup {* add_rewrite_rule @{thm List.nth_Cons'} *}
 
@@ -77,6 +78,7 @@ fun rev_swap :: "'a list \<Rightarrow> nat \<Rightarrow> nat \<Rightarrow> 'a li
   "rev_swap xs i j = (if i < j then rev_swap (list_swap xs i j) (i + 1) (j - 1) else xs)"
 setup {* add_rewrite_rule_cond @{thm rev_swap.simps} [with_filt (size1_filter "i"), with_filt (size1_filter "j")] *}
 setup {* register_wellform_data ("rev_swap xs i j", ["j < length xs"]) *}
+setup {* add_prfstep_check_req ("rev_swap xs i j", "j < length xs") *}
 
 lemma rev_swap_length:
   "j < length xs \<Longrightarrow> length (rev_swap xs i j) = length xs"
@@ -103,7 +105,59 @@ lemma rev_swap_eval [rewrite]:
 @qed
 
 lemma rev_swap_is_rev [rewrite]:
-  "length xs \<ge> 1 \<Longrightarrow> rev_swap xs 0 (length xs - 1) = rev xs"
-@proof @have "length xs - 1 < length xs" @qed
+  "length xs \<ge> 1 \<Longrightarrow> rev_swap xs 0 (length xs - 1) = rev xs" by auto2
+
+section {* take and drop *}
+
+setup {* register_wellform_data ("take n xs", ["n \<le> length xs"]) *}
+setup {* add_prfstep_check_req ("take n xs", "n \<le> length xs") *}
+lemma length_take': "n \<le> length xs \<Longrightarrow> length (take n xs) = n" by simp
+setup {* add_rewrite_rule_cond @{thm length_take'} [with_term "take ?n ?xs"] *}
+lemma nth_take' [rewrite]: "i < length (take n xs) \<Longrightarrow> take n xs ! i = xs ! i" by simp
+setup {* add_rewrite_rule @{thm List.take_0} *}
+
+setup {* add_rewrite_rule_cond @{thm List.length_drop} [with_term "drop ?n ?xs"] *}
+lemma nth_drop' [rewrite]: "i < length (drop n xs) \<Longrightarrow> drop n xs ! i = xs ! (n + i)" by simp
+setup {* add_rewrite_rule @{thm List.drop_0} *}
+
+setup {* add_rewrite_rule @{thm List.append_take_drop_id} *}
+
+section {* Copy one array to the beginning of another *}
+    
+fun array_copy :: "'a list \<Rightarrow> nat \<Rightarrow> 'a list \<Rightarrow> nat \<Rightarrow> nat \<Rightarrow> 'a list" where
+  "array_copy xs i xs' j n =
+    (if n = 0 then xs' else array_copy xs (i + 1) (xs' [j := xs ! i]) (j + 1) (n - 1))"
+setup {* add_rewrite_rule_cond @{thm array_copy.simps} [with_filt (size1_filter "i"), with_filt (size1_filter "j")] *}
+setup {* register_wellform_data ("array_copy xs i xs' j n", ["i + n \<le> length xs", "j + n \<le> length xs'"]) *}
+setup {* add_prfstep_check_req ("array_copy xs i xs' j n", "i + n \<le> length xs \<and> j + n \<le> length xs'") *}
+
+lemma array_copy_length:
+  "i + n \<le> length xs \<Longrightarrow> j + n \<le> length xs' \<Longrightarrow> length (array_copy xs i xs' j n) = length xs'"
+@proof
+  @strong_induct n arbitrary i j xs'
+  @case "n = 0"
+  @apply_induct_hyp "n - 1" "i + 1" "j + 1" "xs' [j := xs ! i]"
+@qed
+setup {* add_forward_prfstep_cond @{thm array_copy_length} [with_term "array_copy ?xs ?i ?xs' ?j ?n"] *}
+
+lemma nat_sub6 [rewrite]: "(a::nat) + (b + 1) - (c + 1) = a + b - c" by simp
+
+lemma array_copy_eval [rewrite]:
+  "i + n \<le> length xs \<Longrightarrow> j + n \<le> length xs' \<Longrightarrow> (array_copy xs i xs' j n) ! k =
+   (if k < j then xs' ! k else if k \<ge> j + n then xs' ! k else xs ! (k + i - j))"
+@proof
+  @strong_induct n arbitrary i j xs'
+  @case "n = 0" @then
+  @apply_induct_hyp "n - 1" "i + 1" "j + 1" "xs' [j := xs ! i]"
+@qed
+
+setup {* del_prfstep_thm @{thm array_copy.simps} *}
+
+lemma array_copy_take [backward]:
+  "n \<le> length xs' \<Longrightarrow> n \<le> length xs \<Longrightarrow> take n (array_copy xs 0 xs' 0 n) = take n xs"
+@proof
+  @have "length (array_copy xs 0 xs' 0 n) = length xs'"
+  @have "length (take n (array_copy xs 0 xs' 0 n)) = length (take n xs)"
+@qed
 
 end
