HOL/SepLogic/DynamicArray.thy
@@ -38,11 +38,16 @@ fun array_copy :: "'a::heap array \<Rightarrow> nat \<Rightarrow> 'a array \<Rig
      })"
 declare array_copy.simps [sep_proc_defs]
 
+setup {* add_rewrite_rule @{thm Reverse_Func.array_copy.simps} *}
 theorem array_copy_rule [hoare_triple, hoare_create_case]:
   "<src \<mapsto>\<^sub>a lsrc * dst \<mapsto>\<^sub>a ldst * \<up>(si + len \<le> length lsrc) * \<up>(di + len \<le> length ldst)>
     array_copy src si dst di len
-   <\<lambda>_. src \<mapsto>\<^sub>a lsrc * dst \<mapsto>\<^sub>a list_update_range ldst di (take len (drop si lsrc))>"
-@proof @induct len arbitrary si di ldst @qed
+   <\<lambda>_. src \<mapsto>\<^sub>a lsrc * dst \<mapsto>\<^sub>a Reverse_Func.array_copy lsrc si ldst di len>"
+@proof @strong_induct len arbitrary si di ldst
+  @case "len = 0"
+  @apply_induct_hyp "len - 1" "si + 1" "di + 1" "list_update ldst di (lsrc ! si)"
+@qed
+setup {* del_prfstep_thm @{thm Reverse_Func.array_copy.simps} *}
 
 definition ensure_length :: "nat \<Rightarrow> 'a::heap dynamic_array \<Rightarrow> 'a dynamic_array Heap" where
   "ensure_length nl d = (case d of
@@ -55,7 +60,9 @@ definition ensure_length :: "nat \<Rightarrow> 'a::heap dynamic_array \<Rightarr
 declare ensure_length_def [sep_proc_defs]
 
 theorem ensure_length_rule [hoare_triple]:
-  "<dyn_array xs p> ensure_length nl p <\<lambda>r. dyn_array xs r * \<up>(amax r \<ge> nl)>\<^sub>t" by auto2
+  "<dyn_array xs p>
+   ensure_length nl p
+   <\<lambda>r. dyn_array xs r * \<up>(amax r \<ge> nl)>\<^sub>t" by auto2
 
 definition push_array :: "'a \<Rightarrow> 'a::heap dynamic_array \<Rightarrow> 'a dynamic_array Heap" where
   "push_array x d = (case d of
@@ -127,7 +134,7 @@ definition array_swap :: "'a::heap dynamic_array \<Rightarrow> nat \<Rightarrow>
     return ()
    }"
 declare array_swap_def [sep_proc_defs]
-declare [[print_trace]]
+
 theorem array_swap_rule [hoare_triple, hoare_create_case]:
   "<dyn_array xs p * \<up>(i < length xs) * \<up>(j < length xs)>
    array_swap p i j
